okay, commit while its sort of working

src/tactic/tactify.lean
@@ -1,18 +1,96 @@
 import tactic
 import data.nat.factorial
 
-open tactic expr
+open tactic
+
+namespace expr
+
+/-- Implementation of `get_app_fn_with_implicits`. -/
+meta def app_implicits : expr → list expr → expr → expr
+| f (x :: xs) (pi _ binder_info.default _ ty) := f
+| f (x :: xs) (pi _ _ _ ty) := app_implicits (f x) xs ty
+| f _ _ := f
+
+/--
+Extract the topmost function along with
+all implicit arguments before the first explicit argument.
+-/
+meta def get_app_fn_with_implicits (e : expr) : tactic expr :=
+let (f, args) := e.get_app_fn_args in
+app_implicits f args <$> infer_type f
+
+/-- Implementation of `app_implicits_mvars`. -/
+meta def app_implicits_mvars_aux : expr → expr → tactic expr
+| f (pi _ binder_info.default _ _) := return f
+| f (pi _ _ v_ty b_ty) := do v ← mk_meta_var v_ty, app_implicits_mvars_aux (f v) b_ty
+| f _ := return f
+
+/-- Fill any implicit arguments in with fresh metavariables. -/
+meta def app_implicits_mvars (e : expr) : tactic expr :=
+infer_type e >>= app_implicits_mvars_aux e
+
+-- /-- Implementation of `app_implicits_placeholders`. -/
+-- meta def app_implicits_placeholders_aux : expr → expr → tactic expr
+-- | f (pi _ binder_info.default _ _) := return f
+-- | f (pi _ _ v_ty b_ty) :=
+--   do app_implicits_placeholders_aux (f (unchecked_cast pexpr.mk_placeholder)) b_ty
+-- | f _ := return f
+
+-- /-- Fill any implicit arguments in with fresh metavariables. -/
+-- meta def app_implicits_placeholders (e : expr) : tactic expr :=
+-- infer_type e >>= app_implicits_placeholders_aux e
+
+meta def lam_binding_names : expr → list name
+| (lam n _ _ b) := n :: lam_binding_names b
+| _ := []
+
+meta def fill_args_with_mvars : expr → tactic expr
+| e := do
+  ty ← infer_type e,
+  match ty with
+  | (pi _ _ t _) := do
+    m ← mk_meta_var t,
+    fill_args_with_mvars $ e m
+  | _ := return e
+  end
+
+meta def replace_args_with_mvars (e : expr) : tactic expr :=
+e.get_app_fn.fill_args_with_mvars
+
+end expr
+
+open expr
 
 namespace tactic
+
+/--
+Create a `tactic_state` with the given `goal` as its goal.
+We don't try particularly hard to "start fresh".
+-/
+meta def tactic_state_with_goal (goal : expr) : tactic tactic_state :=
+lock_tactic_state $ do
+  n ← mk_fresh_name,
+  assert n goal,
+  g :: _ ← get_goals,
+  set_goals [g],
+  local_context >>= (λ ctx, ctx.mmap' (λ h, try (clear h))),
+  get_state
+
+meta def run_with_goal (goal : expr) {α} (t : tactic α) : tactic α :=
+do
+  state ← tactic_state_with_goal goal,
+  run_with_state state t
+
+
 
 namespace tactify
 
 meta inductive proof_step
 | apply (e : expr) : proof_step
 | exact (e : expr) : proof_step
-| intro (n : name) : proof_step
+| intros (ns : list name) : proof_step
 | rewrite (r : expr) : proof_step
-| «sorry» : proof_step
+| «sorry» (comment : format) : proof_step
 
 meta inductive proof_script
 | done : proof_script
@@ -21,19 +99,27 @@ meta inductive proof_script
 namespace proof_step
 
 meta def to_format : proof_step → tactic format
-| (apply e) := do p ← pp e, return format!"apply {p}"
+| (apply e) := do p ← pp e.replace_mvars, return format!"apply {p}"
 | (exact e) := do p ← pp e, return format!"exact {p}"
-| (intro n) := return format!"intro {n}"
+| (intros ns) := do match ns with
+  | [] := fail "unreachable code"
+  | [n] := return format!"intro {n}"
+  | _ := do let ns := string.intercalate " " (ns.map name.to_string), return format!"intros {ns}"
+  end
 | (rewrite r) := do p ← pp r, return format!"rw {p}"
-| («sorry») := return format!"sorry"
+| («sorry» c) := return $ format!"sorry" ++ " -- " ++ c
 
 meta instance : has_to_tactic_format proof_step :=
 ⟨to_format⟩
 
+/--
+Given a list of solutions for the current goals, run a tactic `t`,
+and compute the corresponding solutions for the new goals, if possible.
+-/
 meta def subgoals' (solutions : list expr) {α} (t : tactic α) :
   tactic (list expr) :=
 do
-  -- Keep a copy of the initial goals (which should unify with the solutions)
+  -- Keep a copy of the initial goals.
   initial_goals ← get_goals,
   -- Run the tactic
   -- trace_state,
@@ -41,8 +127,7 @@ do
   t,
   -- trace_state,
   -- trace_result,
-  -- Collect the subgoals
-  get_goals >>= set_goals,
+  -- then collect the new goals.
   new_goals ← get_goals,
   lock_tactic_state $ (do
     -- By unifying the initial goals with the given solutions,
@@ -53,10 +138,11 @@ do
 meta def as_tactic : proof_step → tactic unit
 | (apply e) := tactic.apply e >> skip
 | (exact e) := tactic.exact e
-| (intro n) := tactic.intro n >> skip
-| (rewrite r) := tactic.rewrite_target r >> skip
-| («sorry») := tactic.admit
+| (intros ns) := tactic.intro_lst ns >> skip
+| (rewrite r) := tactic.rewrite_target r >> try reflexivity
+| («sorry» c) := tactic.admit
 
+/-- Update a list of solutions for the current goals, as we progress through a proof_step. -/
 meta def subgoals (solutions : list expr) (step : proof_step) :
   tactic (list expr) :=
 subgoals' solutions step.as_tactic
@@ -76,6 +162,17 @@ meta def to_format : proof_script → tactic format
 meta instance : has_to_tactic_format proof_script :=
 ⟨to_format⟩
 
+/--
+Return a list of pairs, consisting of a proof state, e.g.,
+```
+m n : ℕ,
+h : m ≤ n
+⊢ m.factorial ≤ n.factorial
+```
+and a tactic to run in that state, e.g. `apply nat.le_of_dvd`.
+
+The intended purpose of this view is to generate training data.
+-/
 meta def prompts : proof_script → tactic (list (string × string))
 | (proof_script.done) := return []
 | (proof_script.step st s r) := do
@@ -86,28 +183,21 @@ meta def prompts : proof_script → tactic (list (string × string))
 
 end proof_script
 
-meta def tactic_state_with_goal (goal : expr) : tactic tactic_state :=
-lock_tactic_state $ do
-  n ← mk_fresh_name,
-  assert n goal,
-  g :: _ ← get_goals,
-  set_goals [g],
-  get_state
 
-meta def run_with_goal (goal : expr) {α} (t : tactic α) : tactic α :=
-do
-  state ← tactic_state_with_goal goal,
-  run_with_state state t
-
-/--
-Hopefully `apply f` works against the `state`, in which case return `f`.
-Otherwise, try using `apply f _`, `apply f _ _` and so on.
--/
-meta def apply_with_underscores : expr → tactic expr
-| f := do
-  (lock_tactic_state (tactic.apply f) >> return f) <|>
-  (do f' ← to_expr ``(%%f _),
-      apply_with_underscores f')
+meta def construct_apply_step (e : expr) : tactic proof_step :=
+-- This part just doesn't work. :-(
+-- (do
+--   tgt ← target,
+--   e' ← i_to_expr_strict ``(%%e : %%tgt),
+--   lock_tactic_state (tactic.exact e'),
+--   return (proof_step.exact e')) <|>
+(do
+  lock_tactic_state (tactic.apply e),
+  return (proof_step.apply e)) <|>
+(do
+  pp_e ← pp e,
+  pp_t ← infer_type e >>= pp,
+  return (proof_step.sorry format!"tried to `apply {pp_e}` with type `{pp_t}` but couldn't make it work"))
 
 /--
 Attempt to deduce a single proof step from a list of `solutions` for the current goals,
@@ -118,25 +208,38 @@ meta def tactify_1 (solutions : list expr) :
 do
   let sol := solutions.head,
   s ← match sol with
-  | (const n l) := return (proof_step.exact sol)
-  | (local_const u p b t) := return (proof_step.exact sol)
-  | (lam n bi ty bd) := return (proof_step.intro n) -- TODO use `intros`?
+  | (const _ _) := return (proof_step.exact sol)
+  | (local_const _ _ _ _) := return (proof_step.exact sol)
+  | (lam n _ _ _) := return (proof_step.intros sol.lam_binding_names)
   | (app f x) := do
       let f' := f.get_app_fn,
       match f' with
       | `(@bit0) := return (proof_step.exact sol)
       | `(@bit1) := return (proof_step.exact sol)
       | `(@eq.mpr) := do
+          -- Assume the solution was built using `rw`, and hope we get it right:
           let b := sol.app_fn.app_arg.app_arg.app_arg,
           let b := if b.get_app_fn.const_name = `propext then b.app_arg else b,
           return (proof_step.rewrite b)
+      -- | `(@iff.mpr) := do
+      --     -- Rather than produce separate steps `apply iff.mpr` and then `apply F`,
+      --     -- try to produce `refine (F _ _).mpr` in one step.
+      --     match sol with
+      --     | `(iff.mpr %%F %%x) := do
+      --       -- Since we're playing with `_`s here, we need to discard extra goals that get created.
+      --       -- gs ← get_goals,
+      --       F' ← replace_args_with_mvars F,
+      --       e ← lock_tactic_state $ to_expr ``(iff.mpr %%F'),
+      --       -- set_goals gs,
+      --       return (proof_step.apply e)
+      --     | _ := fail "unreachable code"
+      --     end
       | _ := do
           let n := f'.const_name,
-          if (`dcases_on).is_suffix_of n ∨ (`cases_on).is_suffix_of n then do
-            return (proof_step.sorry)
+          if (`dcases_on).is_suffix_of n ∨ (`cases_on).is_suffix_of n then
+            return (proof_step.sorry "tactify can not cope with cases/induction/pattern mattching")
           else do
-            f'' ← apply_with_underscores f',
-            return (proof_step.apply f'')
+            construct_apply_step f'
       end
   | _ := do
       trace_state,
@@ -190,21 +293,57 @@ meta def tactic_prompts (n : name) : tactic unit := do
     run_with_goal d.type (do
     o ← tactic.tactify [d.value],
     s ← o.prompts,
-    s.mmap' (λ p, do trace p.1, trace p.2, trace ""))
+    s.mmap' (λ p, do trace "---", trace p.1, trace p.2))
+
+meta def all_tactic_prompts : tactic unit := do
+  env ← get_env,
+  env.mfold () (λ d _, do trace d.to_name, try (tactic_prompts d.to_name), trace "==="),
+  skip
+
+-- run_cmd all_tactic_prompts
+-- set_option pp.all true
 
 -- Examples that work:
 run_cmd tactic_prompts `nat.factorial_le
 run_cmd tactic_prompts `nat.units_eq_one
-run_cmd tactic_prompts `nat.add_factorial_succ_lt_factorial_add_succ
 run_cmd tactic_prompts `nat.lt_factorial_self
 run_cmd tactic_prompts `nat.zero_eq_mul
 
+def foo (n m : ℕ) (h : m < n) : m.succ ≤ n :=
+(nat.succ_le_iff).mpr h
+
+run_cmd tactic_prompts `foo
+
+-- TODO combine `apply iff.mpr` and `apply F` into `apply F.mpr`. (also `.mp`)
+run_cmd tactic_prompts `nat.add_factorial_succ_lt_factorial_add_succ
+
+example (i n : ℕ) (hi : 2 ≤ i) : i + n < (i + n) * (i + n).factorial :=
+begin
+  apply iff.mpr (lt_mul_iff_one_lt_right _),
+end
+
+-- TODO Use `exact` insteaf of `apply` where possible?
+run_cmd tactic_prompts `multiset.coe_card -- verify that we generate `exact rfl`, not `apply rfl`.
+
+-- TODO what's going on with
+run_cmd tactic_prompts `add_cancel_comm_monoid.add_comm
+
+-- TODO don't generate `apply id` steps
+run_cmd tactic_prompts `list.decidable_chain._proof_2
+#print list.decidable_chain
+-- TODO avoid `apply id_rhs α`
 -- TODO try generating shorter `rw` proofs (i.e. leave off arguments when they aren't needed)
--- TODO combine `apply iff.mpr` and `apply F` into `apply F.mpr`.
+-- TODO Also `eq.symm` (e.g. `functor.map_map`)?
+-- TODO don't use `Exists.intro`?
 
 -- PROJECT I don't know how to handle proofs that use `cases`, `induction`, or pattern matching.
 run_cmd tactic_prompts `nat.add_factorial_le_factorial_add
 run_cmd tactic_prompts `nat.self_le_factorial
+
+
+#print add_lt_add_of_lt_of_le
+
+#print rfl
 
 example : false :=
 begin
@@ -212,53 +351,109 @@ begin
   tactify `nat.add_factorial_succ_lt_factorial_add_succ,
 end
 
--- Extracted from nat.add_factorial_succ_lt_factorial_add_succ.
-example : ∀ {i : ℕ} (n : ℕ), 2 ≤ i → i + (n + 1).factorial < (i + n + 1).factorial :=
+example {i : ℕ} (n : ℕ) (hi : 2 ≤ i) :
+  i + (n + 1).factorial < (i + n) * (i + n).factorial + (i + n).factorial :=
 begin
-  intro i,
-  intro n,
-  intro hi,
-  rw (i + n).factorial_succ,
-  rw (i + n).succ_eq_add_one,
-  rw add_mul (i + n) 1 (i + n).factorial,
-  rw one_mul (i + n).factorial,
   apply add_lt_add_of_lt_of_le,
   apply has_le.le.trans_lt,
   apply nat.le.intro,
-  apply rfl,
-  exact n,
-  apply iff.mpr,
-  apply lt_mul_iff_one_lt_right,
-  apply has_lt.lt.trans_le,
-  apply zero_lt_two,
-  apply has_le.le.trans,
-  exact hi,
-  apply nat.le.intro,
-  apply rfl,
-  apply iff.mpr,
-  apply lt_iff_le_and_ne,
-  apply and.intro,
-  apply nat.factorial_pos,
-  intro g,
-  apply nat.not_succ_le_self,
-  apply has_le.le.trans,
-  apply has_le.le.trans,
-  exact hi,
-  apply nat.le.intro,
-  apply rfl,
-  exact n,
-  apply iff.mp,
-  apply nat.factorial_eq_one,
-  apply eq.symm,
-  exact g,
-  apply nat.factorial_le,
-  apply has_le.le.trans,
-  apply le_of_eq,
-  apply add_comm,
-  apply iff.mpr,
-  apply add_le_add_iff_right,
-  apply has_le.le.trans,
-  apply one_le_two,
-  exact hi,
-  done,
+  exact rfl,
+  skip,
+end
+
+-- Extracted from nat.add_factorial_succ_lt_factorial_add_succ.
+example : ∀ {i : ℕ} (n : ℕ), 2 ≤ i → i + (n + 1).factorial < (i + n + 1).factorial :=
+begin
+intros i n hi,
+rw (i + n).factorial_succ,
+rw (i + n).succ_eq_add_one,
+rw add_mul (i + n) 1 (i + n).factorial,
+rw one_mul (i + n).factorial,
+apply add_lt_add_of_lt_of_le,
+apply has_le.le.trans_lt,
+apply nat.le.intro,
+apply rfl,
+exact n,
+apply iff.mpr,
+apply lt_mul_iff_one_lt_right,
+apply has_lt.lt.trans_le,
+apply zero_lt_two,
+apply has_le.le.trans,
+exact hi,
+apply nat.le.intro,
+apply rfl,
+apply iff.mpr,
+apply lt_iff_le_and_ne,
+apply and.intro,
+apply nat.factorial_pos,
+intro g,
+apply nat.not_succ_le_self,
+apply has_le.le.trans,
+apply has_le.le.trans,
+exact hi,
+apply nat.le.intro,
+apply rfl,
+exact n,
+apply iff.mp,
+apply nat.factorial_eq_one,
+apply eq.symm,
+exact g,
+apply nat.factorial_le,
+apply has_le.le.trans,
+apply le_of_eq,
+apply add_comm,
+apply iff.mpr,
+apply add_le_add_iff_right,
+apply has_le.le.trans,
+apply one_le_two,
+exact hi,
+done
+end
+
+example : ∀ {i : ℕ} (n : ℕ), 2 ≤ i → i + (n + 1).factorial < (i + n + 1).factorial :=
+begin
+intros i n hi,
+rw (i + n).factorial_succ,
+rw (i + n).succ_eq_add_one,
+rw add_mul (i + n) 1 (i + n).factorial,
+rw one_mul (i + n).factorial,
+apply add_lt_add_of_lt_of_le,
+apply has_le.le.trans_lt,
+apply nat.le.intro,
+apply rfl,
+exact n,
+apply iff.mpr,
+apply lt_mul_iff_one_lt_right,
+apply has_lt.lt.trans_le,
+apply zero_lt_two,
+apply has_le.le.trans,
+exact hi,
+apply nat.le.intro,
+apply rfl,
+apply iff.mpr,
+apply lt_iff_le_and_ne,
+apply and.intro,
+apply nat.factorial_pos,
+intro g,
+apply nat.not_succ_le_self,
+apply has_le.le.trans,
+apply has_le.le.trans,
+exact hi,
+apply nat.le.intro,
+apply rfl,
+exact n,
+apply iff.mp,
+apply nat.factorial_eq_one,
+apply eq.symm,
+exact g,
+apply nat.factorial_le,
+apply has_le.le.trans,
+apply le_of_eq,
+apply add_comm,
+apply iff.mpr,
+apply add_le_add_iff_right,
+apply has_le.le.trans,
+apply one_le_two,
+exact hi,
+done
 end
